src/BinEncoders/Env/Examples/IPv4Header.v
@@ -117,6 +117,49 @@ Proof.
   rewrite H; reflexivity.
 Qed.
 
+Lemma IPv4_Packet_Header_Len_OK
+  : forall ip4 (ctx ctx' ctx'' : CacheEncode) c b b'' ext,
+    (encode_word_Spec (natToWord 4 4)
+    ThenC encode_nat_Spec 4 (IPv4_Packet_Header_Len ip4)
+    ThenC encode_unused_word_Spec 8 (* TOS Field! *)
+    ThenC encode_word_Spec ip4!"TotalLength"
+    ThenC encode_word_Spec ip4!"ID"
+    ThenC encode_unused_word_Spec 1 (* Unused flag! *)
+    ThenC encode_bool_Spec ip4!"DF"
+    ThenC encode_bool_Spec ip4!"MF"
+    ThenC encode_word_Spec ip4!"FragmentOffset"
+    ThenC encode_word_Spec ip4!"TTL"
+    ThenC encode_enum_Spec ProtocolTypeCodes ip4!"Protocol"
+    DoneC) ctx ↝ (b, ctx') ->
+    (encode_word_Spec ip4!"SourceAddress"
+    ThenC encode_word_Spec ip4!"DestAddress"
+    ThenC encode_list_Spec encode_word_Spec ip4!"Options"
+    DoneC) ctx' ↝ (b'', ctx'') ->
+    IPv4_Packet_OK ip4 ->
+    (fun _ => 128) ip4 + (fun a => 16 + |ip4!"Options"| * 32) ip4 + (bin_measure transform_id) + 16 = IPv4_Packet_encoded_measure (transform (transform b (transform (encode_checksum _ _ _ 16 c) b'')) ext).
+Proof.
+  intros.
+  set (k := transform_id); simpl in k; subst k.
+  simpl bin_measure.
+  rewrite length_ByteString_id.
+  unfold IPv4_Packet_encoded_measure.
+  pose proof transform_assoc as H'; simpl in H';
+    rewrite <- !H'.
+  eapply computes_to_compose_decode_unused_word in H;
+    let H' := fresh in
+    destruct H as [? [? [? H'] ] ]; rewrite H'.
+  unfold DecodeBindOpt, If_Opt_Then_Else.
+  eapply computes_to_compose_decode_word in H;
+    let H' := fresh in
+    destruct H as [? [? [? H'] ] ]; rewrite H'.
+  unfold fst.
+  rewrite wordToNat_natToWord_idempotent; try reflexivity;
+    eauto using IPv4_Packet_Headiner_Len_Bound.
+  unfold IPv4_Packet_Header_Len.
+  rewrite Mult.mult_plus_distr_l.
+  omega.
+Qed.
+
 Hint Resolve IPv4_Packet_Header_Len_eq : data_inv_hints.
 
 
@@ -127,54 +170,11 @@ Definition EthernetHeader_decoder
   : CorrectDecoderFor IPv4_Packet_OK encode_IPv4_Packet_Spec.
 Proof.
   start_synthesizing_decoder.
-  intro H; eapply compose_IPChecksum_encode_correct';
-    [apply H
-    | repeat resolve_Checksum
-    | cbv beta; unfold Domain; simpl;
-      repeat calculate_length_ByteString
-    | cbv beta; unfold Domain; simpl;
-      repeat calculate_length_ByteString
-    | solve_mod_8
-    | solve_mod_8
-    |
-    | repeat (decode_step; unfold Domain; simpl)
-    |
-    | instantiate (1 := fun _ _ => True);
-      simpl; intros; exact I | repeat (decode_step; unfold Domain; simpl) ];
-    cbv beta;
-    unfold Domain; simpl.
-  { (* Grossest Proof By Far. *)
-    intros.
-    set (k := transform_id); simpl in k; subst k.
-    rewrite length_ByteString_ByteString_id.
-    instantiate (1 := IPv4_Packet_encoded_measure).
-    unfold IPv4_Packet_encoded_measure.
-    pose proof transform_assoc as H'; simpl in H';
-    rewrite <- !H'.
-    eapply computes_to_compose_decode_unused_word in H0;
-      let H' := fresh in
-      destruct H0 as [? [? [? H'] ] ]; rewrite H'.
-    unfold DecodeBindOpt, If_Opt_Then_Else.
-    eapply computes_to_compose_decode_word in H0;
-      let H' := fresh in
-      destruct H0 as [? [? [? H'] ] ]; rewrite H'.
-    unfold fst.
-    rewrite wordToNat_natToWord_idempotent; try reflexivity;
-      eauto using IPv4_Packet_Headiner_Len_Bound.
-    unfold IPv4_Packet_Header_Len.
-    rewrite Mult.mult_plus_distr_l.
-    clear.
-    repeat match goal with
-             |- context [length ?l] => remember (length l)
-           end.
-    assert (n = n0) by (rewrite Heqn, Heqn0; f_equal).
-    rewrite H.
-    omega. }
-
-  simpl.
-  unfold IPv4_Packet_OK; clear; intros ? H'; destruct H' as [? ?]; repeat split.
-  simpl.
-  unfold IPv4_Packet_Header_Len.
+  normalize_compose transformer.
+  apply_IPChecksum IPv4_Packet_Header_Len_OK.
+  
+  simpl; unfold IPv4_Packet_OK; clear; intros ? H'; destruct H' as [? ?]; repeat split.
+  simpl; unfold IPv4_Packet_Header_Len.
   revert H; unfold StringId11; unfold pow2, mult; simpl; auto with arith.
 
   repeat (decode_step; unfold Domain; simpl).
@@ -184,12 +184,8 @@ Proof.
 
 Defined.
 
-(* This is the decoder function that we should extract. *)
-
 Definition IPv4_decoder_impl :=
   Eval simpl in (fst (proj1_sig EthernetHeader_decoder)).
-
-Print IPv4_decoder_impl.
 
 Definition pkt' : list char :=
   [WO~1~0~1~0~0~0~1~0;
@@ -225,29 +221,21 @@ Definition pkt' : list char :=
 Definition pkt : list char :=
     Eval compute in map (@natToWord 8) [69;0;100;0;0;0;0;0;38;1;243;159;192;168;222;10;192;168;222;1;0;0;0;0].
 
-
-  Compute (InternetChecksum.checksum pkt).
+Compute (InternetChecksum.checksum pkt).
 
 Definition address : list char :=
   Eval compute in map (@natToWord 8) [172;16;254;1].
 
-Print address.
 Lemma zero_lt_eight : (lt 0 8)%nat.
-  Proof. omega. Qed.
+Proof. omega. Qed.
 
-  Definition blah
-    := {| padding := 0; front := WO; paddingOK := zero_lt_eight; byteString := address |}.
+Definition fiat_ipv4_decode (buffer: list char) : option (IPv4_Packet * list char) :=
+  let bs := {| padding := 0; front := WO; paddingOK := zero_lt_eight; byteString := buffer |} in
+  match IPv4_decoder_impl bs () with
+  | Some (pkt', bs, _) => Some (pkt', bs.(byteString))
+  | None => None
+  end.
 
-  Definition fiat_ipv4_decode (buffer: list char) : option (IPv4_Packet * list char) :=
-    let bs := {| padding := 0; front := WO; paddingOK := zero_lt_eight; byteString := buffer |} in
-    match IPv4_decoder_impl bs () with
-    | Some (pkt', bs, _) => Some (pkt', bs.(byteString))
-    | None => None
-    end.
+Compute (fiat_ipv4_decode pkt).
 
-  (* Decoder works on hand-written packet copied from tutorial, so
-   it's got that going for it. (well, except that the total length
-   field in the example was ill-formed :p) *)
-  Compute (fiat_ipv4_decode pkt).
-
-  Compute (InternetChecksum.checksum pkt).
+Compute (InternetChecksum.checksum pkt).
